Hoare sound proof complete

hoareProofDefScript.sml
@@ -16,9 +16,9 @@ End
 Inductive Hoare:
   (Hoare P CSkip P) ∧
   (Hoare (assert_subst Q v ae) (CAsgn v ae) Q) ∧
-  (Hoare P c1 Q ∧ Hoare Q c2 R ⇒ Hoare P (Cseq c1 c2) R) ∧
-  (Hoare (λenv. P env ∧ eval_expr env b T) c1 Q ∧
-   Hoare (λenv. P env ∧ eval_expr env b F) c2 Q ⇒ Hoare P (CIf b c1 c2) Q) ∧  
+  (Hoare P c1 Q ∧ Hoare Q c2 R ⇒ Hoare P (CSeq c1 c2) R) ∧
+  (Hoare (λenv. P env ∧ eval_bexpr env b T) c1 Q ∧
+   Hoare (λenv. P env ∧ eval_bexpr env b F) c2 Q ⇒ Hoare P (CIf b c1 c2) Q) ∧  
   (Hoare (λenv. P env ∧ eval_bexpr env b T) c P ⇒ Hoare P (CWhile b c) (λenv. P env ∧ (eval_bexpr env b F))) ∧ 
   (∀ P1 Q1. (∀ env. P0 env ⇒ P1 env) ∧ Hoare P1 c Q1 ∧ (∀ env. Q1 env ⇒ Q0 env) ⇒ Hoare P0 c Q0)
 End
@@ -52,11 +52,16 @@ Proof
   >-(simp [is_valid_def, assert_subst_def, Once eval_com_cases]
      >> rw[] >> first_x_assum drule >> simp[])
   (* Seq *)
-  >-(cheat)
+  >-(fs[is_valid_def] >> simp[Once eval_com_cases] >> rw[] >> gs[]
+     >> qpat_x_assum ‘∀env0 env1. P env0 ∧ eval_com env0 c1 env1 ⇒ Q env1’ drule_all
+     >> rw[] >> first_x_assum irule >> qexists_tac ‘env2’ >> gs[])
   (* If *)
-  >-(cheat)
+  >-(fs[is_valid_def] >> simp[Once eval_com_cases] >> rw[]
+     >-(last_x_assum (qspecl_then [‘env0’, ‘env1’] assume_tac) >> fs[])
+     >-(first_x_assum (qspecl_then [‘env0’, ‘env1’] assume_tac) >> fs[]))
   (* While *)
-  >-(cheat)
+  >-(fs[is_valid_def] >> Induct_on ‘eval_com’ >> rw[]
+     >> first_x_assum drule_all >> gs[])
   (* Consequence *)
   (*  >-(fs[is_valid_def] >> metis_tac[]) works, but the following is more step-by-step approach. *)
   >-(fs[is_valid_def] >>  drule_all hoare_consequence_pre >> drule_all hoare_consequence_post  >> rw[]
